rr_frontend/radium/src/specs.rs
@@ -720,7 +720,11 @@ impl TyOwnSpec {
 
     #[must_use]
     pub fn fmt_shared(&self, tid: &str, lft: &str) -> String {
-        format!("{} ◁ₗ[{}, Shared {}] #({}) @ (◁ {})", self.loc, tid, lft, self.rfn, self.ty)
+        if self.with_later {
+            format!("guarded ({} ◁ₗ[{}, Shared {}] #({}) @ (◁ {}))", self.loc, tid, lft, self.rfn, self.ty)
+        } else {
+            format!("{} ◁ₗ[{}, Shared {}] #({}) @ (◁ {})", self.loc, tid, lft, self.rfn, self.ty)
+        }
     }
 }
 
