case_studies/minivec/output/minivec/proofs/proof_Vec_T_len.v
@@ -17,7 +17,7 @@ Proof.
   all: print_remaining_goal.
   Unshelve. all: sidecond_solver.
   Unshelve. all: sidecond_hammer.
-  rewrite Hlen_eq project_vec_els_length. lia. 
+  rewrite Hlen_eq project_vec_els_length. lia.
   Unshelve. all: print_remaining_sidecond.
 Qed.
 End proof.
