theories/rust_typing/shims.v
@@ -276,8 +276,8 @@ Proof.
     ls_count ◁ₗ[π, Owned false] PlaceIn (Z.of_nat i) @ (◁ int usize_t) ∗
     ls_src ◁ₗ[π, Owned false] PlaceIn l_s @ (◁ alias_ptr_t) ∗
     ls_dst ◁ₗ[π, Owned false] PlaceIn l_t @ (◁ alias_ptr_t) ∗
-    l_s ◁ₗ[ π, Owned false] # (fmap (M:=list) PlaceIn (reshape (replicate len (ly_size T_st_ly)) v_s)) @ (◁ array_t (value_t (UntypedSynType T_st_ly)) len) ∗
-    l_t ◁ₗ[π, Owned false] #(fmap (M:=list) PlaceIn (take i (reshape (replicate len (ly_size T_st_ly)) v_s) ++ drop i (reshape (replicate len (ly_size T_st_ly)) v_t))) @ (◁ array_t (value_t (UntypedSynType T_st_ly)) len)))%I).
+    l_s ◁ₗ[ π, Owned false] # (fmap (M:=list) PlaceIn (reshape (replicate len (ly_size T_st_ly)) v_s)) @ (◁ array_t len (value_t (UntypedSynType T_st_ly))) ∗
+    l_t ◁ₗ[π, Owned false] #(fmap (M:=list) PlaceIn (take i (reshape (replicate len (ly_size T_st_ly)) v_s) ++ drop i (reshape (replicate len (ly_size T_st_ly)) v_t))) @ (◁ array_t len (value_t (UntypedSynType T_st_ly)))))%I).
   iApply (typed_goto_acc _ _ _ _ _ loop_inv).
   { unfold_code_marker_and_compute_map_lookup. }
   liRStep; liShow. iExists 0%nat.
@@ -437,14 +437,14 @@ Definition type_of_ptr_copy `{RRGS : !refinedrustGS Σ} (T_rt : Type) (T_st : sy
     (l, off_src) :@: offset_ptr_t T_st,
     (l, off_dst) :@: offset_ptr_t T_st,
     count :@: int usize_t; λ π,
-    (l ◁ₗ[π, Owned false] (#xs) @ (◁ array_t (maybe_uninit T_ty) len)) ∗
+    (l ◁ₗ[π, Owned false] (#xs) @ (◁ array_t len (maybe_uninit T_ty))) ∗
     ⌜(0 ≤ count)%Z⌝ ∗
     ⌜0 ≤ off_src⌝ ∗
     ⌜0 ≤ off_dst⌝ ∗
     ⌜(off_src + count < len)%Z⌝ ∗
     ⌜(off_dst + count < len)%Z⌝)
   → ∃ () : unit, () @ unit_t; λ π,
-    l ◁ₗ[π, Owned false] (#(ptr_copy_result off_src off_dst (Z.to_nat count) xs)) @ (◁ array_t (maybe_uninit T_ty) len).
+    l ◁ₗ[π, Owned false] (#(ptr_copy_result off_src off_dst (Z.to_nat count) xs)) @ (◁ array_t len (maybe_uninit T_ty)).
 
 Lemma ptr_copy_typed `{RRGS : !refinedrustGS Σ} π (T_rt : Type) (T_st : syn_type) (T_ly : layout) :
   syn_type_has_layout T_st T_ly →
